\documentclass{article}
\usepackage{amsmath}
\usepackage{xrf}

\begin{document}

\section*{Linear System Example}
Unknowns: $x$, $y$, $z$. Named constants: $\namel{alpha}{\alpha}$, $\namel{beta}{\beta}$, $\namel{gamma}{\gamma}$.
Right-hand side constants: $\constl{c1}$, $\constl{c2}$, $\constl{c3}$.

\begin{align}
\terml{t:eq1} = x + \namer{alpha}y + \namer{beta}z &= \constr{c1} \\
\terml{t:eq2} = y + \namer{gamma}z &= \constr{c2} \\
\terml{t:eq3} = z &= \constr{c3}
\end{align}

From \termr{t:eq3} we get $z$ immediately. Using \termr{t:eq2} and substituting \termr{t:eq3}:
\begin{align}
y &= \constr{c2} - \namer{gamma}\,\constr{c3}.
\end{align}
Using \termr{t:eq1} and substituting the expressions from \termr{t:eq2} and \termr{t:eq3}:
\begin{align}
x &= \constr{c1} - \namer{alpha}\,\constr{c2} + (\namer{alpha}\namer{gamma} - \namer{beta})\constr{c3}.
\end{align}

Therefore, the solved system is:
\begin{align}
z &= \constr{c3}, \\
y &= \constr{c2} - \namer{gamma}\,\constr{c3}, \\
x &= \constr{c1} - \namer{alpha}\,\constr{c2} + (\namer{alpha}\namer{gamma} - \namer{beta})\constr{c3}.
\end{align}

\end{document}
